Clean up context equiv. stuff a bit

linking/CompositionalComplements.v
@@ -33,169 +33,64 @@ Definition mk_tgt_sem (tp : Asm_module) :=
   let tge := Genv.globalenv tp in
   @Modsem.mk Asm_comp.fundef unit tge Asm_coop.state (Asm_eff.Asm_eff_sem hf).
 
-(** Apply the contextual equivalence functor from
-   linking/context_equiv.v to to linking/linking_proof.v.*)
+(** Apply the contextual equivalence functor from [linking/context_equiv.v] to
+[linking/linking_proof.v]. *)
 
 Module CE := ContextEquiv LinkingSimulation.
 
-Section CompositionalComplements.
-
+Lemma compcert_equiv  
 (** There are [N] modules. *)
-
-Variable N : pos.
+  (N : pos)
 
 (** Source and target modules. ['I_N -> A], for [A : Type], is the type of finite
- functions from [{0..N-1}] to [A]. *)
-
-Variable source_modules : 'I_N -> Clight_module.
-Variable target_modules : 'I_N -> Asm_module.
+  functions from [{0..N-1}] to [A]. *)
+  (source_modules : 'I_N -> Clight_module)
+  (target_modules : 'I_N -> Asm_module)
 
 (** The function [plt] maps a subset of the possible function names to the
   modules in which they are defined. *)
-
-Variable plt : ident -> option 'I_N.
+  (plt : ident -> option 'I_N) :
 
 (** Wrap the source and target modules as 'Modsem's (as in Section 3). *)
-
-Definition sems_S (ix : 'I_N) := mk_src_sem (source_modules ix).
-Definition sems_T (ix : 'I_N) := mk_tgt_sem (target_modules ix).
+  let sems_S (ix : 'I_N) := mk_src_sem (source_modules ix) in
+  let sems_T (ix : 'I_N) := mk_tgt_sem (target_modules ix) in
+  let prog_S := Prog.mk sems_S in
+  let prog_T := Prog.mk sems_T in
 
 (** [ge_top] and the two [domeq_*] hypotheses below constrain the source--target
   global envs. of the modules in [sems_S] and [sems_T] to have equal domain, as
   explained in Section 3. *)
+  forall ge_top : ge_ty,
+  forall domeq_S : (forall ix : 'I_N, genvs_domain_eq ge_top (sems_S ix).(Modsem.ge)),
+  forall domeq_T : (forall ix : 'I_N, genvs_domain_eq ge_top (sems_T ix).(Modsem.ge)), 
 
-Variable ge_top : ge_ty.
-Variable domeq_S : forall ix : 'I_N, genvs_domain_eq ge_top (sems_S ix).(Modsem.ge).
-Variable domeq_T : forall ix : 'I_N, genvs_domain_eq ge_top (sems_T ix).(Modsem.ge). 
+(** No module defines the same module twice. *)
+  forall lnr : (forall ix : 'I_N, list_norepet (map fst (prog_defs (source_modules ix)))),
 
 (** The target modules are (independently) compiled from the respective
   source modules ([transf_clight_program] compiles Clight programs to Asm). *)
+  forall transf : 
+    (forall ix : 'I_N, transf_clight_program (source_modules ix) 
+                     = Errors.OK (target_modules ix)),
 
-Variable transf : 
-  forall ix : 'I_N, 
-  transf_clight_program (source_modules ix) 
-  = Errors.OK (target_modules ix).
+(** All of the above together imply that [prog_S] and [prog_T] are contextually
+  equivalent. *) 
+  Equiv_ctx ge_top plt prog_S prog_T.
 
-(** Here we just prove that compilation preserves the set of global symbols. *)
-
-Lemma find_syms :
+Proof.
+move=> sems_S sems_T prog_S prog_T ge_top deqS deqT lnr transf.
+have find_syms :
   forall (i : 'I_N) (id : ident) (bf : block),
   Genv.find_symbol (Modsem.ge (sems_S i)) id = Some bf ->
   Genv.find_symbol (Modsem.ge (sems_T i)) id = Some bf.
-Proof.
-intros idx id bf.
-unfold sems_S, sems_T; simpl.
-generalize (transf idx); intros H.
-apply transf_clight_program_preserves_syms with (s := id) in H.
-rewrite H; auto.
+{ move=> idx id bf; rewrite /sems_S /sems_T /=; move: (transf idx)=> H.
+  by apply transf_clight_program_preserves_syms with (s := id) in H; rewrite H. }
+apply: CE.equiv=> //.
+by move=> ix; apply: Clight_RC.
+by move=> ix; apply: Asm_is_nuc.
+move=> ix; rewrite /Prog.sems/= => m m' m'' ge c c' c'' /= H H2. 
+by eapply asm_step_det; eauto.
+move=> ix; move: (transf ix)=> H.
+by eapply transf_clight_program_correct in H; eauto.
 Qed.
-
-(** The (deterministic) context [C]. Assumptions on [C] are: 
-- [sim_C]: C self-simulates ([C <= C]) (cf. Definition 2, pg. 10). 
-- [det_C]: C is deterministic (cf. Definition 2, pg. 10). This is true,
-      e.g., of all Clight and assembly contexts. 
-- [rclosed_C] restricts to reach-closed contexts (cf. linking/rc_semantics.v).
-- [nuke_C] restricts contexts to those that store only valid blocks.  This is
-      footnote 5 on pg. 9 of the paper (one reviewer suggested we describe this
-      condition in a bit more detail in the paper; we tend to agree and plan to
-      do so in the final version). It turns out that this condition holds of all
-      assembly contexts; see backend/Asm_nucular.v for the proof. 
-- [domeq_C]: The global environment attached to the [C] module semantics 
-      has the same domain (set of blocks marked "global") as [ge_top]. *)
-
-Variable C : Modsem.t.   
-Variable sim_C : 
-  SM_simulation.SM_simulation_inject 
-  C.(Modsem.sem) C.(Modsem.sem) C.(Modsem.ge) C.(Modsem.ge).
-Variable rclosed_C : RCSem.t (Modsem.sem C) (Modsem.ge C).
-Variable nuke_C : Nuke_sem.t (Modsem.sem C).
-Variable det_C : semantics_lemmas.corestep_fun (Modsem.sem C).
-Variable domeq_C : genvs_domain_eq ge_top C.(Modsem.ge).
-
-Notation source_linked_semantics := (CE.linker_S sems_S plt C).
-Notation target_linked_semantics := (CE.linker_T sems_T plt C).
-
-Definition safe ge l m := 
-  forall n, closed_safety.safeN source_linked_semantics ge n l m.
-
-
-
-Lemma clight_modules_rclosed (ix : 'I_N) : 
-  RCSem.t (Modsem.sem (sems_S ix)) (Modsem.ge (sems_S ix)).
-Proof. solve[apply (Clight_RC hf)]. Qed.
-
-Lemma asm_modules_nucular (ix : 'I_N) : Nuke_sem.t (Modsem.sem (sems_T ix)).
-Proof. solve[apply Asm_is_nuc]. Qed.
-
-(** The [init] hypothesis just ensures that no module defines the same function
-  twice. *)
-
-Variable lnr : forall ix : 'I_N, 
-  list_norepet (map fst (prog_defs (source_modules ix))).
-
-(** Here we prove that [S_i <= T_i] for each source/target module pair, using
-  Theorem [transf_clight_program_correct] from
-  driver/CompositionalCompiler.v. *)
-
-Lemma modules_inject (ix : 'I_N) : 
-  SM_simulation.SM_simulation_inject 
-    (Modsem.sem (sems_S ix)) (Modsem.sem (sems_T ix)) 
-    (Modsem.ge (sems_S ix)) (Modsem.ge (sems_T ix)).
-Proof.
-generalize (transf ix); intros H.
-eapply transf_clight_program_correct in H; eauto.
-Qed.
-
-(** The entry point for the linked program: *)
-
-Variable main : Values.val.
-
-(** * Contextual Equivalence in Matching States *)
-
-(** Starting from matching source--target states, the source/target programs
- equiterminate when linked with [C], assuming the source linked program is safe
- and reach-closed (see above).  This is Corollary 2 on pg. 11 of the paper. *)
-
-Notation lifted_sim := 
-  (CE.lifted_sim clight_modules_rclosed asm_modules_nucular 
-   plt modules_inject domeq_S domeq_T 
-   find_syms sim_C domeq_C rclosed_C nuke_C main).
-
-Theorem context_equiv cd mu l1 m1 l2 m2 
-  (source_safe : safe ge_top l1 m1) 
-  (match12 : Wholeprog_sim.match_state lifted_sim cd mu l1 m1 l2 m2) :
-  (terminates source_linked_semantics ge_top l1 m1 
-   <-> terminates target_linked_semantics ge_top l2 m2).
-Proof. 
-eapply CE.context_equiv; eauto.   
-unfold CE.extend_sems; intros ix; destruct (lt_dec ix N); auto.
-simpl; intros m m' m'' ge c c' c'' H H2. 
-simpl in H, H2; eapply asm_step_det; eauto.
-Qed.
-
-(** * Contextual Equivalence in Initial States *)
-
-(** The following corollary (really, of CE.context_equiv) specializes
-  to entry point main and the initial state of the linked program. *)
-
-Theorem init_context_equiv l1 m1 m2 j vals1 vals2
-  (source_safe : safe ge_top l1 m1)
-  (init1 : initial_core source_linked_semantics ge_top main vals1 = Some l1)
-  (init1_inv : cc_init_inv j ge_top vals1 m1 ge_top vals2 m2) :
-  exists l2, 
-  [/\ initial_core target_linked_semantics ge_top main vals2 = Some l2
-    & (terminates source_linked_semantics ge_top l1 m1 
-   <-> terminates target_linked_semantics ge_top l2 m2)].
-Proof. 
-eapply CE.init_context_equiv; eauto.
-apply: clight_modules_rclosed.
-apply: asm_modules_nucular.
-apply: modules_inject.
-apply: find_syms.
-unfold CE.extend_sems; intros ix; destruct (lt_dec ix N); auto.
-simpl; intros m m' m'' ge c c' c'' H H2. 
-simpl in H, H2; eapply asm_step_det; eauto.
-Qed.
-
-End CompositionalComplements.
   
