linking/context_equiv.v
@@ -7,6 +7,7 @@ Require Import pos.
 Require Import compcert_linking.
 Require Import rc_semantics.
 Require Import rc_semantics_lemmas.
+Require Import context.
 Require Import linking_spec.
 
 (* ssreflect *)
@@ -22,49 +23,25 @@ Require Import closed_simulations_lemmas.
 Require Import closed_safety.
 Require Import semantics_lemmas.
 
-Import Wholeprog_sim.
 Import SM_simulation.
+Import Wholeprog_sim.
 Import Linker. 
 Import Modsem.
 
-(** * Reach-Closed Contextual Equivalence *)
-
-Module ContextEquiv (LS : LINKING_SIMULATION).                  
-                                                                       
-Import LS.                                                             
-                                                                       
 Lemma pos_incr' (p : pos) : (0 < (p+1))%nat.                           
 Proof. omega. Qed.                                                     
                                                                        
 Definition pos_incr (p : pos) := mkPos (pos_incr' p).                  
 
-Section ContextEquiv.
+Module Prog.
+Record t (N : pos) : Type := mk {sems :> 'I_N -> Modsem.t}.
+End Prog.
 
-Variable (N0 : pos) (sems_S0 sems_T0 : 'I_N0 -> Modsem.t).
+Section ExtendSems.
 
-Variable rclosed_S0 : forall ix : 'I_N0, RCSem.t (sems_S0 ix).(sem) (sems_S0 ix).(ge).
-Variable nucular_T0 : forall ix : 'I_N0, Nuke_sem.t (sems_T0 ix).(sem).
-
-Variable plt0 : ident -> option 'I_N0.
-Variable sims0 : forall ix : 'I_N0,                                          
-                 let s := sems_S0 ix in                                              
-                 let t := sems_T0 ix in                                              
-                 SM_simulation_inject s.(sem) t.(sem) s.(ge) t.(ge).
-
-Variable ge_top : ge_ty.                                                     
-Variable domeq_S0 : forall ix : 'I_N0, genvs_domain_eq ge_top (sems_S0 ix).(ge).
-Variable domeq_T0 : forall ix : 'I_N0, genvs_domain_eq ge_top (sems_T0 ix).(ge). 
-
-Variable find_symbol_ST : 
-  forall (i : 'I_N0) id bf, 
-  Genv.find_symbol (ge (sems_S0 i)) id = Some bf -> 
-  Genv.find_symbol (ge (sems_T0 i)) id = Some bf.
-
-Variable C : Modsem.t.   
-Variable sim_C : SM_simulation_inject C.(sem) C.(sem) C.(ge) C.(ge).
-Variable domeq_C : genvs_domain_eq ge_top C.(ge).
-Variable rclosed_C : RCSem.t (sem C) (ge C).
-Variable nuke_C : Nuke_sem.t (sem C).
+Variable ge : ge_ty.
+Variable C : Ctx.t ge.
+Variable N0 : pos.
 
 Let N := pos_incr N0.
 
@@ -74,145 +51,96 @@ Proof. by move=> H; apply/ssrnat.ltP. Qed.
 Definition extend_sems (f : 'I_N0 -> Modsem.t) (ix : 'I_N) : Modsem.t :=
   match lt_dec ix N0 with
     | left pf => let ix' : 'I_N0 := Ordinal (lt_ssrnatlt pf) in f ix'
-    | right _ => C
+    | right _ => C.(Ctx.C)
   end.
 
-(** [sems_S] extends the source semantics with context [C], by mapping all
-functions that are not defined by any of the modules in [sems_S0] to [C]
-(cf. [extend_sems] above). *)
+End ExtendSems.
 
-Let sems_S := extend_sems sems_S0.
+(** * Reach-Closed Contextual Equivalence *)
 
-(** [sems_T] does the same for the target semantics [sems_T0]. *)
+Definition apply_ctx (ge : ge_ty) (C : Ctx.t ge) 
+                     (N : pos) (p : Prog.t N) : Prog.t (pos_incr N) :=
+  Prog.mk (extend_sems C p.(Prog.sems)).
 
-Let sems_T := extend_sems sems_T0.
+Lemma leq_N_Nincr (N : pos) : ssrnat.leq N (pos_incr N).
+Proof. by rewrite /= plus_comm. Qed.
 
-Lemma find_symbol_ST' : 
-  forall (i : 'I_N) id bf, 
-  Genv.find_symbol (ge (sems_S i)) id = Some bf -> 
-  Genv.find_symbol (ge (sems_T i)) id = Some bf.
+Lemma leq_SN_Nincr (N : pos) : ssrnat.leq (S N) (pos_incr N).
+Proof. by rewrite /= plus_comm. Qed.
+
+Definition link_ctx (ge : ge_ty) (C : Ctx.t ge) (N : pos) (p : Prog.t N) plt : EffectSem :=
+  let extended_plt (id : ident) := 
+    match plt id with
+      | None => Some (Ordinal (leq_SN_Nincr N))
+      | Some ix => Some (widen_ord (leq_N_Nincr N) ix)
+    end
+  in effsem (pos_incr N) (Prog.sems (apply_ctx C p)) extended_plt.
+
+Definition Terminates G C M (sem : CoreSemantics G C M) (ge : G) (m : M) 
+                      (main : val) (args : list val) :=
+  forall c, initial_core sem ge main args = Some c -> terminates sem ge c m.
+
+Definition Equiv_ctx (ge : ge_ty) (N : pos) plt (p1 p2 : Prog.t N) :=
+  forall C : Ctx.t ge,
+  forall (main : val) (args1 args2 : list val) m1 m2,
+  forall c1, initial_core (link_ctx C p1 plt) ge main args1 = Some c1 -> 
+  forall j, cc_init_inv j ge args1 m1 ge args2 m2 -> 
+  (forall n, safeN (link_ctx C p1 plt) ge n c1 m1) -> 
+      (Terminates (link_ctx C p1 plt) ge m1 main args1 
+   <-> Terminates (link_ctx C p2 plt) ge m2 main args2).
+
+(** Prove that Simulation implies Equiv_ctx *)
+
+Module ContextEquiv (LS : LINKING_SIMULATION). 
+                                                                       
+Import LS.                                                             
+                                                                       
+Section ContextEquiv.
+
+Variable N : pos.
+Variable pS pT : Prog.t N.
+Variable rclosed_S : forall ix : 'I_N, RCSem.t (Prog.sems pS ix).(sem) (Prog.sems pS ix).(ge).
+Variable valid_T : forall ix : 'I_N, Nuke_sem.t (Prog.sems pT ix).(sem).
+Variable targets_det : forall ix : 'I_N, corestep_fun (Prog.sems pT ix).(sem).
+Variable plt : ident -> option 'I_N.
+Variable sims : 
+  forall ix : 'I_N,                                          
+  let s := Prog.sems pS ix in                                              
+  let t := Prog.sems pT ix in                                              
+  SM_simulation_inject s.(sem) t.(sem) s.(ge) t.(ge).
+Variable ge_top : ge_ty.                                                     
+Variable domeq_S : forall ix : 'I_N, genvs_domain_eq ge_top (Prog.sems pS ix).(ge).
+Variable domeq_T : forall ix : 'I_N, genvs_domain_eq ge_top (Prog.sems pT ix).(ge). 
+Variable find_symbol_ST : 
+  forall (ix : 'I_N) id bf, 
+  Genv.find_symbol (ge (Prog.sems pS ix)) id = Some bf -> 
+  Genv.find_symbol (ge (Prog.sems pT ix)) id = Some bf.
+
+Lemma equiv : Equiv_ctx ge_top plt pS pT.
 Proof.
-rewrite /sems_S /sems_T /extend_sems=> i id bf.
-by case: (lt_dec i N0)=> // pf; apply: find_symbol_ST.
-Qed.
-
-Lemma sims (ix : 'I_N) :
-  let s := sems_S ix in
-  let t := sems_T ix in
-  SM_simulation_inject (sem s) (sem t) (ge s) (ge t).
-Proof.
-rewrite /sems_S /sems_T /extend_sems; case e: (lt_dec ix N0)=> [pf|//].
-by apply: (sims0 (Ordinal (lt_ssrnatlt pf))).
-Qed.
-
-Lemma leq_N0_N : ssrnat.leq N0 N.
-Proof. by rewrite /N /= plus_comm. Qed.
-
-Lemma leq_SN0_N : ssrnat.leq (S N0) N.
-Proof. by rewrite /N /= plus_comm. Qed.
-
-(** [plt] is the new procedure table equal to [plt0] on [dom(plt0)], but which
-otherwise maps function [id]s to the module index assigned to the context
-[C]. *)
-
-Definition plt (id : ident) := 
-  match plt0 id with
-    | None => Some (Ordinal leq_SN0_N)
-    | Some ix => Some (widen_ord leq_N0_N ix)
-  end.
-
-(** [linker_S] and [linker_T] define the extended source--target semantics,
-resp., in which [sems_S0] and [sems_T0] are linked with the context [C]. *)
-
-Definition linker_S := effsem N sems_S plt.
-
-Definition linker_T := effsem N sems_T plt.
-
-Lemma rclosed_S (ix : 'I_N) : RCSem.t (sem (sems_S ix)) (ge (sems_S ix)).
-Proof. by rewrite /sems_S /extend_sems; case e: (lt_dec ix N0). Qed.
-
-Lemma nucular_T (ix : 'I_N) : Nuke_sem.t (sem (sems_T ix)).
-Proof. by rewrite /sems_T /extend_sems; case e: (lt_dec ix N0). Qed.
-
-(** Prove the existence of pairwise simulations between source and target 
-module semantics in the extended semantics. *)
-
-Lemma sm_inject (ix : 'I_N) :
- let s := sems_S ix in
- let t0 := sems_T ix in
- SM_simulation_inject (sem s) (sem t0) (ge s) (ge t0).
-Proof.
-rewrite /= /sems_S /sems_T /extend_sems; case e: (lt_dec _ _)=> [//|].
-by apply: sim_C.
-Qed.
-
-Lemma genvs_domeq_S (ix : 'I_N) : genvs_domain_eq ge_top (ge (sems_S ix)).
-Proof. 
-rewrite /sems_S /extend_sems; case e: (lt_dec _ _)=> [//|].
-by apply: domeq_C.
-Qed.
-
-Lemma genvs_domeq_T (ix : 'I_N) : genvs_domain_eq ge_top (ge (sems_T ix)).
-Proof. 
-rewrite /sems_T /extend_sems; case e: (lt_dec _ _)=> [//|].
-by apply: domeq_C.
-Qed.
-
-(** [lifted_sim] proves a closed simulation on the source and target programs,
-after they are (independently) linked with the context [C]. *)
-
-Lemma lifted_sim (main : val) :
-  CompCert_wholeprog_sim linker_S linker_T ge_top ge_top main.
-Proof.
-apply: link=> //. 
-by apply: find_symbol_ST'.
-by apply: rclosed_S.
-by apply: nucular_T.
-by apply: sm_inject.
-by apply: genvs_domeq_S.
-by apply: genvs_domeq_T.
-Qed.
-
-Import Wholeprog_sim.
-
-(** ** Proof of Corollary 1 *)
-
-Lemma context_equiv 
-    (main : val)  
-    (targets_det : forall ix : 'I_N, corestep_fun (sem (sems_T ix))) 
-    cd mu l1 m1 l2 m2 
-    (source_safe : forall n, safeN linker_S ge_top n l1 m1) 
-    (match12 : match_state (lifted_sim main) cd mu l1 m1 l2 m2) :
-  (terminates linker_S ge_top l1 m1 <-> terminates linker_T ge_top l2 m2).
-Proof.
-have target_det: corestep_fun linker_T by apply: linking_det.
-by apply (equitermination _ _ target_det _ _ _ _ _ _ source_safe match12).
-Qed.
-
-(** ** Corollary 1, Specialized to Initial States *)
-
-Lemma init_context_equiv l1 m1 m2 j vals1 vals2 
-  (main : val)
-  (targets_det : forall ix : 'I_N, corestep_fun (sem (sems_T ix))) 
-  (source_safe : forall n, closed_safety.safeN linker_S ge_top n l1 m1)
-  (init1 : initial_core linker_S ge_top main vals1 = Some l1)
-  (init1_inv : cc_init_inv j ge_top vals1 m1 ge_top vals2 m2) :
-  exists l2, 
-  [/\ initial_core linker_T ge_top main vals2 = Some l2 
-    & (terminates linker_S ge_top l1 m1 <-> terminates linker_T ge_top l2 m2)].
-Proof.
+rewrite /Equiv_ctx=> C main args1 args2 m1 m2 c1 Init1 j Inv. 
+have sim: CompCert_wholeprog_sim (link_ctx C pS plt) (link_ctx C pT plt) ge_top ge_top main.
+{ apply: link=> ix; rewrite /Prog.sems/apply_ctx/extend_sems. 
+  by move=> ??; case e: (lt_dec ix N)=> [pf|pf] //; apply find_symbol_ST.
+  by case e: (lt_dec ix N)=> [pf|pf] //; apply: (Ctx.rclosed_C C).
+  by case e: (lt_dec ix N)=> [pf|pf] //; apply: (Ctx.valid_C C).
+  by case e: (lt_dec ix N)=> [pf|pf] //; apply: (Ctx.sim_C C).
+  by case e: (lt_dec ix N)=> [pf|pf] //; apply: (Ctx.domeq_C C).
+  by case e: (lt_dec ix N)=> [pf|pf] //; apply: (Ctx.domeq_C C). }
+have target_det: corestep_fun (link_ctx C pT plt). 
+{ apply: linking_det=> ix; rewrite /Prog.sems/apply_ctx/extend_sems.
+  by case e: (lt_dec ix N)=> [pf|pf] //; apply Ctx.det_C. }
+move: (Init1)=> Init1' Hsafe.
 eapply @core_initial 
-  with (Sem1 := linker_S) (Sem2 := linker_T) 
-       (ge1 := ge_top) (ge2 := ge_top) 
-       (halt_inv := cc_halt_inv)
-       (j := j)
-       (main := main)
-       (m1 := m1)
-       (m2 := m2)
-       (w := lifted_sim main)
-  in init1; eauto.
-case init1=> mu []cd []c2 []H []H2 H3; exists c2; split=> //.
-eapply context_equiv; eauto.
+  with (Sem1 := link_ctx C pS plt) (Sem2 := link_ctx C pT plt) 
+       (ge1 := ge_top) (ge2 := ge_top) (halt_inv := cc_halt_inv)
+       (j := j) (main := main) (m1 := m1) (m2 := m2) (w := sim)
+  in Init1; eauto.
+case: Init1=> mu []cd []c2 []_ []Init2 Hmatch.
+apply equitermination in Hmatch=> //. 
+split=> Hterm x Init.
+{ by rewrite Init2 in Init; case: Init=> <-; rewrite -Hmatch; apply: Hterm. }
+{ by rewrite Init1' in Init; case: Init=> <-; rewrite Hmatch; apply: Hterm. }
 Qed.
 
 End ContextEquiv.
