linking/context.v
@@ -1,0 +1,42 @@
+(* sepcomp imports *)
+
+Require Import sepcomp. Import SepComp. 
+Require Import arguments.
+
+(* ssreflect *)
+
+Require Import ssreflect ssrbool ssrfun seq eqtype fintype.
+Set Implicit Arguments.
+Unset Strict Implicit.
+Unset Printing Implicit Defensive.
+
+Require Import pos.
+Require Import rc_semantics.
+Require Import nucular_semantics.
+Require Import compcert_linking. Import Modsem.
+Require Import simulations. Import SM_simulation.
+Require Import semantics_lemmas.
+
+(** The (deterministic) context [C]. Assumptions on [C] are: 
+- [sim_C]: C self-simulates ([C <= C]) (cf. Definition 2, pg. 10). 
+- [det_C]: C is deterministic (cf. Definition 2, pg. 10). This is true,
+      e.g., of all Clight and assembly contexts. 
+- [rclosed_C] restricts to reach-closed contexts (cf. linking/rc_semantics.v).
+- [nuke_C] restricts contexts to those that store only valid blocks.  This is
+      footnote 5 on pg. 9 of the paper (one reviewer suggested we describe this
+      condition in a bit more detail in the paper; we tend to agree and plan to
+      do so in the final version). It turns out that this condition holds of all
+      assembly contexts; see backend/Asm_nucular.v for the proof. 
+- [domeq_C]: The global environment attached to the [C] module semantics 
+      has the same domain (set of blocks marked "global") as [ge_top]. *)
+
+Module Ctx. 
+Record t (ge_top : ge_ty) : Type := {
+    C : Modsem.t
+  ; sim_C : SM_simulation_inject C.(sem) C.(sem) C.(ge) C.(ge)
+  ; rclosed_C : RCSem.t (sem C) (ge C)
+  ; valid_C : Nuke_sem.t (sem C)
+  ; det_C : corestep_fun (sem C)
+  ; domeq_C : genvs_domain_eq ge_top (ge C)
+  }.
+End Ctx.
