Makefile
@@ -168,7 +168,8 @@ LINKING=cast.v pos.v stack.v seq_lemmas.v pred_lemmas.v \
   sepcomp.v gallina_coresem.v inj_lemmas.v join_sm.v reestablish.v wf_lemmas.v\
   linking_spec.v linking.v compcert_linking.v compcert_linking_lemmas.v \
   disjointness.v reach_lemmas.v rc_semantics.v rc_semantics_lemmas.v \
-  linking_inv.v ret_lemmas.v call_lemmas.v linking_proof.v context_equiv.v \
+  linking_inv.v ret_lemmas.v call_lemmas.v linking_proof.v \
+  context.v context_equiv.v \
   jstep.v safe_clight_rc.v CompositionalComplements.v 
 
 # Putting everything together (in driver/)
